

Introduction to University Mathematics

MATH40001/MATH40009

Solutions to Mid-module Test

1. **Total: 20 Marks**

- (a) i) Show that for all $n \in \mathbb{N}$, $n \neq \nu(n)$.
Let $A = \{n \in \mathbb{N} | n \neq \nu(n)\}$. Obviously $0 \in A$, since $0 \neq \nu(0)$, by axiom (P3). Assume $n \in A$, then $n \neq \nu(n)$, but this means by injectivity of ν (axiom (P4)), that $\nu(n) \neq \nu(\nu(n))$, hence $\nu(n) \in A$, and $A = \mathbb{N}$ by axiom (P5).
- ii) Show that for all $n, m \in \mathbb{N}$, $n \neq \nu(n + m)$.
Let $A = \{n \in \mathbb{N} | n \neq \nu(n + m), \forall m \in \mathbb{N}\}$. $0 \in A$ as $0 \neq \nu(m)$ for all m in \mathbb{N} . Assume $n \in A$, then $n \neq \nu(n + m), \forall m \in \mathbb{N}$. We want to show $\nu(n) \in A$. Assume $\nu(n) = \nu(\nu(n) + m)$ for some m , but then by axiom (P4), $n = \nu(n) + m = m + \nu(n) = \nu(n + m)$, by commutativity of addition and definition of addition. This contradicts the induction hypothesis. Therefore $\nu(n) \in A$, and $A = \mathbb{N}$.
- iii) Conclude that for all $n, m \in \mathbb{N}$ nonzero, $n \neq n + m$.
Since m is nonzero, $m = \nu(k)$ for some k , by Problem Sheet 1. Now $n + m = n + \nu(k) = \nu(n + k)$. By (ii), we have $n \neq \nu(n + k)$ and hence $n \neq n + m$.
- (b) In this problem, don't use any properties of \leq or $<$, just the definition.
- i) Show that $(m \leq n) \Rightarrow (\nu(m) \leq \nu(n))$.
Suppose $m \leq n$. Then $n = m + u$ for some $u \in \mathbb{N}$ by definition of \leq . By commutativity, $n = u + m$. So $\nu(n) = \nu(u + m) = u + \nu(m)$ by Definition of Addition. By commutativity again, $\nu(n) = \nu(m) + u$. Thus $\nu(m) \leq \nu(n)$.
- ii) Show that the relation \leq is antisymmetric.
First we show that if $n \leq m$ and $m \leq n$, then $n = m$ (the antisymmetry property). Indeed, suppose $u, v \in \mathbb{N}$ satisfy $n = m + u$ and $m = n + v$. Then $n = (n + v) + u$. By associativity this implies $n = n + (v + u)$. This implies that $v + u = 0$: for otherwise, $v + u = \nu(k)$ for some $k \in \mathbb{N}$ (as shown in lectures), and then $n = n + \nu(k)$ which contradicts part (ii) above. But now by a result from lectures again we obtain $v = u = 0$. So then $n = m + 0 = m$ and $n = m$.
- ii) Show that no two of the properties $n < m$ or $n = m$ or $n > m$ can hold.
Now, by definition, $n < m$ implies that $n \neq m$ and similarly $n > m$ implies $n \neq m$. On the other hand, by antisymmetry, $n < m$ and $n > m$ implies $n = m$ but $n \neq m$, a contradiction. So at most one of the three properties above is satisfied.
- (c) Let S be a nonempty subset of \mathbb{Z} . Show that if there exists an element $m \in \mathbb{Z}$ such that for all $x \in S$, $x > m$, then S has a least element.
By definition, for every $x \in S$, there exists $n \in \mathbb{N}$ such that $x = m + n$. Let $A := \{n \in \mathbb{N} | m + n \in S\}$. Since S is nonempty, we have seen that A must also be nonempty. By the well-ordering property, there is a least element $a \in A$. Now we claim that $c := m + a$ is the least element of S . Indeed, for every $x \in S$, $x = m + n$, and we have $n \geq a$ by definition of a . So $n = a + k$ for some $k \in \mathbb{N}$. Finally, $x = m + n = m + (a + k) = (m + a) + k$ where we used the associativity. Hence $x \geq c = m + a$, as desired.

2. **Total: 20 Marks**

- (a) $\gcd(10672, 4147) = 29$.

- (b) i. Show that if n, m and k are nonzero integers, then $k \gcd(m, n) = \gcd(km, kn)$.
 Let $d = \gcd(m, n)$, then $d \mid m, n$, hence $dk \mid km, kn$ and therefore $dk \mid \gcd(km, kn)$.
 Set $\gcd(km, kn) = d' dk$. So $d' dk \mid km, kn$. Hence then $d' d \mid m, n$ and so $d' d \mid \gcd(m, n) = d$, which implies $d' = 1$. Thus $\gcd(km, kn) = d$.
- ii. Show that if $a \equiv b \pmod{m}$, then $ac \equiv bc \pmod{mc}$, for $c > 0$.
 If $a \equiv b \pmod{m}$, then there exists an integer k , such that $a = b + km$. Therefore
 $ac = bc + (km)c = bc + k(mc)$ and by definition of equivalence class modulo mc ,
 $ac \equiv bc \pmod{mc}$.
- (c) Let p be a prime, $p \mid n_1 n_2 \dots n_k$, where n_1, n_2, \dots, n_k are nonzero natural numbers. Then $p \mid n_j$, for some j , such that $1 \leq j \leq k$.
 We prove this by induction. For $k = 1$ the result is trivial. Assume now that the result is true for an arbitrary k . Consider $n_1 n_2 \dots n_{k+1}$ divisible by p . Notice that either $\gcd(p, n_1 n_2 \dots n_k) = 1$ or $\gcd(p, n_1 n_2 \dots n_k) = p$. Now if $\gcd(p, n_1 n_2 \dots n_k) = 1$ then, $p \mid n_{k+1}$ by Euclid's Lemma. But if $p \mid n_1 n_2 \dots n_k$, then by the induction hypothesis, there exists an integer i such that $p \mid n_i$.

3. Total: 20 Marks

- (a) Let \mathbf{a}, \mathbf{b} and \mathbf{c} three vectors in \mathbb{R}^3 . In the standard basis $\{\hat{\mathbf{i}}, \hat{\mathbf{j}}, \hat{\mathbf{k}}\}$, we write $\mathbf{a} = a_1 \hat{\mathbf{i}} + a_2 \hat{\mathbf{j}} + a_3 \hat{\mathbf{k}}$, $\mathbf{b} = b_1 \hat{\mathbf{i}} + b_2 \hat{\mathbf{j}} + b_3 \hat{\mathbf{k}}$ and $\mathbf{c} = c_1 \hat{\mathbf{i}} + c_2 \hat{\mathbf{j}} + c_3 \hat{\mathbf{k}}$.
- i. We know that in a right-handed orthonormal basis, $\hat{\mathbf{i}} \times \hat{\mathbf{j}} = \hat{\mathbf{k}}, \hat{\mathbf{j}} \times \hat{\mathbf{k}} = \hat{\mathbf{i}}$ and $\hat{\mathbf{k}} \times \hat{\mathbf{i}} = \hat{\mathbf{j}}$. We also know that $\hat{\mathbf{j}} \times \hat{\mathbf{i}} = -\hat{\mathbf{k}}, \hat{\mathbf{i}} \times \hat{\mathbf{k}} = -\hat{\mathbf{j}}$ and $\hat{\mathbf{k}} \times \hat{\mathbf{j}} = -\hat{\mathbf{i}}$. As well, we have $\hat{\mathbf{i}} \times \hat{\mathbf{i}} = \hat{\mathbf{j}} \times \hat{\mathbf{j}} = \hat{\mathbf{k}} \times \hat{\mathbf{k}} = 0$. First, we can write directly (or rederive) that

$$\mathbf{b} \times \mathbf{c} = (b_2 c_3 - b_3 c_2) \hat{\mathbf{i}} + (b_3 c_1 - b_1 c_3) \hat{\mathbf{j}} + (b_1 c_2 - b_2 c_1) \hat{\mathbf{k}}$$

So we obtain

$$\begin{aligned} \mathbf{a} \times (\mathbf{b} \times \mathbf{c}) &= [a_1 \hat{\mathbf{i}} + a_2 \hat{\mathbf{j}} + a_3 \hat{\mathbf{k}}] \times [(b_2 c_3 - b_3 c_2) \hat{\mathbf{i}} + (b_3 c_1 - b_1 c_3) \hat{\mathbf{j}} + (b_1 c_2 - b_2 c_1) \hat{\mathbf{k}}] \\ &= (b_2 c_3 - b_3 c_2)(a_3 \hat{\mathbf{j}} - a_2 \hat{\mathbf{k}}) + (b_3 c_1 - b_1 c_3)(a_1 \hat{\mathbf{k}} - a_3 \hat{\mathbf{i}}) + (b_1 c_2 - b_2 c_1)(a_2 \hat{\mathbf{i}} - a_1 \hat{\mathbf{j}}) \\ &= (a_3 b_1 c_3 - a_3 b_3 c_1 + a_2 b_1 c_2 - a_2 b_2 c_1) \hat{\mathbf{i}} + \\ &\quad (a_3 b_2 c_3 - a_3 b_3 c_2 + a_1 b_2 c_1 - a_1 b_1 c_2) \hat{\mathbf{j}} + \\ &\quad (a_2 b_3 c_2 - a_2 b_2 c_3 + a_1 b_3 c_1 - a_1 b_1 c_3) \hat{\mathbf{k}} \end{aligned}$$

If we consider the first component of that vector, we can realize that:

$$\begin{aligned} a_3 b_1 c_3 - a_3 b_3 c_1 + a_2 b_1 c_2 - a_2 b_2 c_1 &= a_1 c_1 b_1 + a_2 c_2 b_1 + a_3 c_3 b_1 - a_1 b_1 c_1 - a_2 b_2 c_1 - a_3 b_3 c_1 \\ &= (a_1 c_1 + a_2 c_2 + a_3 c_3) b_1 - (a_1 b_1 + a_2 b_2 + a_3 b_3) c_1 \\ &= (\mathbf{a} \cdot \mathbf{c}) b_1 - (\mathbf{a} \cdot \mathbf{b}) c_1 \end{aligned}$$

We proceed similarly with the other two components to obtain:

$$\begin{aligned} (\mathbf{a} \times \mathbf{b}) \times \mathbf{c} &= [(\mathbf{a} \cdot \mathbf{c}) b_1 - (\mathbf{a} \cdot \mathbf{b}) c_1] \hat{\mathbf{i}} + [(\mathbf{a} \cdot \mathbf{c}) b_2 - (\mathbf{a} \cdot \mathbf{b}) c_2] \hat{\mathbf{j}} + [(\mathbf{a} \cdot \mathbf{c}) b_3 - (\mathbf{a} \cdot \mathbf{b}) c_3] \hat{\mathbf{k}} \\ &= (\mathbf{a} \cdot \mathbf{c})(b_1 \hat{\mathbf{i}} + b_2 \hat{\mathbf{j}} + b_3 \hat{\mathbf{k}}) - (\mathbf{a} \cdot \mathbf{b})(c_1 \hat{\mathbf{i}} + c_2 \hat{\mathbf{j}} + c_3 \hat{\mathbf{k}}) \\ &= (\mathbf{a} \cdot \mathbf{c}) \mathbf{b} - (\mathbf{a} \cdot \mathbf{b}) \mathbf{c} \end{aligned}$$

5 Marks

- ii. Using the result from the previous question, we can write

$$\begin{aligned} \mathbf{a} \times (\mathbf{b} \times \mathbf{c}) + \mathbf{b} \times (\mathbf{c} \times \mathbf{a}) + \mathbf{c} \times (\mathbf{a} \times \mathbf{b}) &= [(\mathbf{a} \cdot \mathbf{c}) \mathbf{b} - (\mathbf{a} \cdot \mathbf{b}) \mathbf{c}] + [(\mathbf{b} \cdot \mathbf{a}) \mathbf{c} - (\mathbf{b} \cdot \mathbf{c}) \mathbf{a}] + [(\mathbf{c} \cdot \mathbf{b}) \mathbf{a} - (\mathbf{c} \cdot \mathbf{a}) \mathbf{b}] \\ &= (\mathbf{a} \cdot \mathbf{c}) \mathbf{b} - (\mathbf{a} \cdot \mathbf{b}) \mathbf{c} + (\mathbf{a} \cdot \mathbf{b}) \mathbf{c} - (\mathbf{b} \cdot \mathbf{c}) \mathbf{a} + (\mathbf{b} \cdot \mathbf{c}) \mathbf{a} - (\mathbf{c} \cdot \mathbf{a}) \mathbf{b} \\ &= \mathbf{0} \end{aligned}$$

where we have used the symmetry of the dot product.

3 Marks

(b) These two vectors are orthogonal if and only if their scalar product is equal to zero:

$$(3, 2, x) \cdot (2x, 4, x) = 0 \iff x^2 + 6x + 8 = 0 \iff (x+2)(x+4) = 0 \iff x = -2 \text{ or } x = -4$$

3 Marks

(c) Without loss of generality, we set up a coordinate system such that S is at the origin, $R = (0, y_1, 0)$, $Q = (x_2, y_2, 0)$ and $P = (x_3, y_3, z_3)$.

In this coordinate system, we have

$$\begin{aligned}\mathbf{SR} &= (0, y_1, 0), \\ \mathbf{SQ} &= (x_2, y_2, 0), \\ \mathbf{SP} &= (x_3, y_3, z_3), \\ \mathbf{QR} &= (-x_2, y_1 - y_2, 0), \\ \mathbf{QP} &= (x_3 - x_2, y_3 - y_2, z_3).\end{aligned}$$

A vector that is normal to the face opposite vertex S in an outward direction is given by

$$\mathbf{u}_S = \mathbf{QR} \times \mathbf{QP} = (y_1 z_3 - y_2 z_3) \hat{\mathbf{i}} + x_2 z_3 \hat{\mathbf{j}} + (-x_2 y_3 - x_3 y_1 + x_3 y_2 + x_2 y_1) \hat{\mathbf{k}}$$

Similarly, we find that

$$\begin{aligned}\mathbf{u}_R &= \mathbf{SQ} \times \mathbf{SP} = y_2 z_3 \hat{\mathbf{i}} - x_2 z_3 \hat{\mathbf{j}} + (x_2 y_3 - x_3 y_2) \hat{\mathbf{k}} \\ \mathbf{u}_Q &= \mathbf{SP} \times \mathbf{SR} = -y_1 z_3 \hat{\mathbf{i}} + x_3 y_1 \hat{\mathbf{k}} \\ \mathbf{u}_P &= \mathbf{SR} \times \mathbf{SQ} = -x_2 y_1 \hat{\mathbf{k}}\end{aligned}$$

We thus conclude that

$$\mathbf{u}_P + \mathbf{u}_Q + \mathbf{u}_R + \mathbf{u}_S = \mathbf{0}$$

By definition of the cross product, we know that $|\mathbf{u}_P|$ is the area of the parallelogram formed by the vectors \mathbf{SR} and \mathbf{SQ} ; this implies that $|\mathbf{u}_P|$ is twice the area of the triangle QRS . So we conclude that $|\mathbf{u}_P| = 2|\mathbf{u}_1|$, so we get $\mathbf{u}_P = 2\mathbf{u}_1$. We can reason similarly to write that: $\mathbf{u}_Q = 2\mathbf{u}_2$, $\mathbf{u}_R = 2\mathbf{u}_3$ and $\mathbf{u}_S = 2\mathbf{u}_4$. Thus, we conclude that

$$\mathbf{u}_1 + \mathbf{u}_2 + \mathbf{u}_3 + \mathbf{u}_4 = \mathbf{0}$$

(d) In the previous question, we have defined the vector \mathbf{u}_1 to have length equal to the area of the face opposite P , so we can say that $|\mathbf{u}_1| = A$. The direction of \mathbf{u}_1 is perpendicular to the face and pointing outward. Similarly, we can write that $|\mathbf{u}_2| = B$, $|\mathbf{u}_3| = C$ and $|\mathbf{u}_4| = D$.

In the previous question, we concluded that $\mathbf{u}_1 + \mathbf{u}_2 + \mathbf{u}_3 + \mathbf{u}_4 = \mathbf{0}$. So

$$\begin{aligned}\mathbf{u}_4 &= -(\mathbf{u}_1 + \mathbf{u}_2 + \mathbf{u}_3) \Rightarrow |\mathbf{u}_4| = |-(\mathbf{u}_1 + \mathbf{u}_2 + \mathbf{u}_3)| = |\mathbf{u}_1 + \mathbf{u}_2 + \mathbf{u}_3| \\ &\Rightarrow |\mathbf{u}_4|^2 = |\mathbf{u}_1 + \mathbf{u}_2 + \mathbf{u}_3|^2 \\ &\Rightarrow \mathbf{u}_4 \cdot \mathbf{u}_4 = (\mathbf{u}_1 + \mathbf{u}_2 + \mathbf{u}_3) \cdot (\mathbf{u}_1 + \mathbf{u}_2 + \mathbf{u}_3) \\ &\Rightarrow \mathbf{u}_4 \cdot \mathbf{u}_4 = \sum_{i,j=1}^3 \mathbf{u}_i \cdot \mathbf{u}_j\end{aligned}$$

Since the vertex S is trirectangular, we know that the three faces meeting at S are by definition orthogonal to one another, which means that the vectors \mathbf{u}_1 , \mathbf{u}_2 and \mathbf{u}_3 are orthogonal to one another. That means that $\mathbf{u}_i \cdot \mathbf{u}_j = 0$ for $i \neq j$, with $i, j \in \{1, 2, 3\}$. Thus, we are left with

$$\mathbf{u}_4 \cdot \mathbf{u}_4 = \mathbf{u}_1 \cdot \mathbf{u}_1 + \mathbf{u}_2 \cdot \mathbf{u}_2 + \mathbf{u}_3 \cdot \mathbf{u}_3 \Rightarrow |\mathbf{u}_4|^2 = |\mathbf{u}_1|^2 + |\mathbf{u}_2|^2 + |\mathbf{u}_3|^2 \Rightarrow D^2 = A^2 + B^2 + C^2$$